gut receipts out of PagedJournal; proof obligations remain; refinement probably a mess

Splinter/Journal/PagedJournal.i.dfy
@@ -35,22 +35,123 @@ module PagedJournal {
     predicate WF()
     {
       && messageSeq.WF()
+      && (priorRec.Some? ==> 
+        && priorRec.value.WF()
+        && priorRec.value.messageSeq.CanConcat(messageSeq)
+      )
     }
+
+    predicate Valid(boundaryLSN: LSN) {
+      && WF()
+      // If you needed to truncate before you got here, you shouldn't be asking for my I()
+      && boundaryLSN < messageSeq.seqEnd
+      && (|| messageSeq.CanDiscardTo(boundaryLSN)
+          || (priorRec.Some? && priorRec.value.Valid(boundaryLSN))
+         )
+    }
+
+    function I(boundaryLSN: LSN) : (out: MsgHistory)
+      requires Valid(boundaryLSN)
+      ensures out.WF()
+      ensures out.seqStart == boundaryLSN
+      decreases this, 0
+    {
+      if messageSeq.CanDiscardTo(boundaryLSN)
+      then messageSeq.DiscardOld(boundaryLSN) // and don't deref the priorRec!
+      else IOptionJournalRecord(boundaryLSN, priorRec).Concat(messageSeq)
+    }
+
+    lemma NewBoundaryValid(oldLSN: LSN, newLSN: LSN)
+      requires Valid(oldLSN)
+      requires oldLSN <= newLSN
+      requires newLSN < messageSeq.seqEnd
+      ensures Valid(newLSN)
+    {
+      if newLSN < messageSeq.seqStart {
+        priorRec.value.NewBoundaryValid(oldLSN, newLSN);
+      }
+    }
+
+    predicate CanCropHeadRecords(boundaryLSN: LSN, depth: nat)
+    {
+      && Valid(boundaryLSN)
+      && (if depth == 0
+        then true // always okay to return self!
+        else
+          && !(boundaryLSN < messageSeq.seqStart)           // my record isn't last due to boundaryLSN
+          && OptRecCanCropHeadRecords(priorRec, boundaryLSN, depth-1) // I have a priorRec
+        )
+    }
+
+    function CropHeadRecords(boundaryLSN: LSN, depth: nat) : Option<JournalRecord>
+      requires CanCropHeadRecords(boundaryLSN, depth)
+    {
+      if depth == 0
+      then Some(this)
+      else OptRecCropHeadRecords(priorRec, boundaryLSN, depth-1)
+    }
+
+    function MessageSeqAfterCrop(boundaryLSN: LSN, depth: nat) : MsgHistory
+      requires Valid(boundaryLSN)
+      requires CanCropHeadRecords(boundaryLSN, depth+1)
+    {
+      CropHeadRecords(boundaryLSN, depth).value.messageSeq
+    }
+  }
+
+  predicate OptRecCanCropHeadRecords(ojr: Option<JournalRecord>, boundaryLSN: LSN, depth: nat)
+  {
+    if ojr.None?
+    then depth==0
+    else ojr.value.CanCropHeadRecords(boundaryLSN, depth)
+  }
+
+  function OptRecCropHeadRecords(ojr: Option<JournalRecord>, boundaryLSN: LSN, depth: nat) : Option<JournalRecord>
+    requires OptRecCanCropHeadRecords(ojr, boundaryLSN, depth)
+  {
+    if ojr.None?
+    then None
+    else ojr.value.CropHeadRecords(boundaryLSN, depth)
+  }
+
+  lemma OptionNewBoundaryValid(ojr: Option<JournalRecord>, oldLSN: LSN, newLSN: LSN)
+    requires ojr.Some? ==> && ojr.value.Valid(oldLSN)
+    requires ojr.Some? ==> newLSN < ojr.value.messageSeq.seqEnd
+    requires oldLSN <= newLSN
+    ensures ojr.Some? ==> ojr.value.Valid(newLSN)
+  {
+    if ojr.Some? {
+      ojr.value.NewBoundaryValid(oldLSN, newLSN);
+    }
+  }
+
+  function IOptionJournalRecord(boundaryLSN: LSN, ojr: Option<JournalRecord>) : (out: MsgHistory)
+    requires ojr.Some? ==> ojr.value.Valid(boundaryLSN)
+    ensures out.seqStart == boundaryLSN
+    ensures out.seqEnd == if ojr.Some? then ojr.value.messageSeq.seqEnd else boundaryLSN
+    ensures out.WF()
+    decreases ojr, 1
+  {
+      if ojr.None?
+      then EmptyHistoryAt(boundaryLSN)
+      else ojr.value.I(boundaryLSN)
   }
 
   // Recursive "ignorant" discard: throws away old records, but doesn't really
   // have any idea if the records are meaningfully chained; we'll need to assume
   // TJValid later to prove anything about the output of this function.
   function DiscardOldJournalRec(rec: Option<JournalRecord>, lsn: LSN) : (out: Option<JournalRecord>)
+    requires rec.Some? ==> rec.value.Valid(lsn)
+    ensures out.Some? ==> out.value.Valid(lsn)
   {
     if rec.None?
     then None
     else
-      Some(JournalRecord(rec.value.messageSeq,
+      var priorRec := 
         if rec.value.messageSeq.seqStart <= lsn
         then None
-        else DiscardOldJournalRec(rec.value.priorRec, lsn)
-      ))
+        else DiscardOldJournalRec(rec.value.priorRec, lsn);
+      Some(JournalRecord(rec.value.messageSeq, priorRec))
   }
 
   // A TruncatedJournal is some long chain but which we ignore beyond the boundaryLSN
@@ -70,14 +171,8 @@ module PagedJournal {
       TruncatedJournal(boundaryLSN, freshestRec.value.priorRec)
     }
 
-    function BuildReceipt() : Receipt
-    {
-      BuildReceiptRecursive(boundaryLSN, freshestRec)
-    }
-
     predicate WF() {
-      && var receipt := BuildReceipt();
-      && receipt.TJValid()
+      && freshestRec.Some? ==> freshestRec.value.Valid(boundaryLSN)
     }
 
     predicate IsEmpty()
@@ -92,81 +187,36 @@ module PagedJournal {
       if freshestRec.Some? then freshestRec.value.messageSeq.seqEnd else boundaryLSN
     }
 
+    // TODO(tony): LET'S GET I() OUT OF THIS FILE!!!
     function I() : MsgHistory
       requires WF()
+      ensures I().WF()
     {
-      BuildReceipt().I()
+      IOptionJournalRecord(boundaryLSN, freshestRec)
     }
 
     function DiscardOldDefn(lsn: LSN) : (out:TruncatedJournal)
       requires WF()
-      requires I().CanDiscardTo(lsn)
+      requires I().CanDiscardTo(lsn)  // TODO(tony) replace with condition on boundaryLSN / SeqEnd()
+      ensures out.WF()
     {
       TruncatedJournal(lsn,
-        if SeqEnd() <= lsn then None else DiscardOldJournalRec(freshestRec, lsn))
-    }
-
-    function DiscardOld(lsn: LSN) : (out:TruncatedJournal)
-      requires WF()
-      requires I().CanDiscardTo(lsn)
-      ensures out.WF()
-      ensures out.I() == I().DiscardOld(lsn)
-    {
-      var out := DiscardOldDefn(lsn);
-      assert out.WF() && out.I() == I().DiscardOld(lsn) by {
-        var discardReceipt := BuildReceipt().DiscardOld(lsn);
-        out.BuildReceipt().ReceiptsUnique(discardReceipt);
-      }
-      out
+        if SeqEnd() <= lsn then None
+        else
+          OptionNewBoundaryValid(freshestRec, boundaryLSN, lsn);
+          DiscardOldJournalRec(freshestRec, lsn)
+      )
     }
 
     // msgs appears as the (boundary-truncated) contents of the i'th entry in the
-    // receipt
-    predicate IncludesSubseqAt(msgs: MsgHistory, i: nat)
+    // chain of JournalRecords
+    predicate HasMessagesAtDepth(msgs: MsgHistory, depth: nat)
       requires WF()
       requires msgs.WF()
     {
-      && i < |BuildReceipt().lines|
-      // TODO(jonh): Wait, this allows non-truncated inclusions.
-      && BuildReceipt().MessageSeqAt(i).IncludesSubseq(msgs)
-    }
-
-    lemma SubseqOfEntireInterpretation(msgs: MsgHistory, i: nat)
-      requires WF()
-      requires msgs.WF()
-      requires IncludesSubseqAt(msgs, i)
-      ensures I().IncludesSubseq(msgs)
-    {
-      // Propagate subseq relation inductively down the receipt
-      var receipt := BuildReceipt();
-      receipt.TJFacts();
-      var j:=i;
-      assert receipt.OneLinkedInterpretation(j) by { receipt.reveal_LinkedInterpretations(); }
-
-      assert 0<i ==> receipt.InterpretationWF(i-1);
-      while j<|receipt.lines|-1
-        invariant j<|receipt.lines|
-        invariant var jint := receipt.lines[j].interpretation;
-            && jint.Some?
-            && jint.value.WF()
-            && jint.value.IncludesSubseq(msgs)
-      {
-        assert receipt.OneLinkedInterpretation(j+1) by { receipt.reveal_LinkedInterpretations(); }
-        j:=j+1;
-      }
-    }
-
-    lemma LsnBelongs(lsn: LSN)
-      requires BuildReceipt().TJValid()
-      requires boundaryLSN <= lsn < SeqEnd()
-      ensures lsn in BuildReceipt().I().LSNSet()
-      decreases freshestRec
-    {
-      if lsn < Last(BuildReceipt().lines).journalRec.messageSeq.seqStart {
-        // If it's not it in the last journal record, it's gotta be in here
-        // somewhere. Look upstream.
-        prior().LsnBelongs(lsn);
-      }
+      && freshestRec.Some?
+      && freshestRec.value.CanCropHeadRecords(boundaryLSN, depth)
+      && freshestRec.value.MessageSeqAfterCrop(boundaryLSN, depth) == msgs
     }
 
     function AppendRecord(msgs: MsgHistory) : (out: TruncatedJournal)
@@ -176,587 +226,21 @@ module PagedJournal {
       this.(freshestRec := Some(JournalRecord(msgs, freshestRec)))
     }
 
-    function FreezeOffRecent(keepReceiptLines: nat) : (out: TruncatedJournal)
-      requires WF()
-      requires keepReceiptLines <= |BuildReceipt().lines|
-      ensures out.WF()
+    function CropHeadRecords(depth: nat) : TruncatedJournal
     {
-      var out := TruncatedJournal(boundaryLSN,
-        if keepReceiptLines==0 then None
-        else Some(BuildReceipt().lines[keepReceiptLines-1].journalRec));
-      assert out.WF() by {
-        BuildReceipt().SnipAtTJValid(keepReceiptLines);
-        out.BuildReceipt().ReceiptsUnique(BuildReceipt().SnipAt(keepReceiptLines));
-      }
-      out
+      TruncatedJournal(boundaryLSN, OptRecCropHeadRecords(freshestRec, boundaryLSN, depth))
     }
 
-    predicate FreezeForCommit(frozenJournal: TruncatedJournal, keepReceiptLines: nat)
+    predicate FreezeForCommit(frozenJournal: TruncatedJournal, depth: nat)
       requires WF()
     {
       && frozenJournal.WF()
-      && keepReceiptLines <= |BuildReceipt().lines|
-      && boundaryLSN <= frozenJournal.boundaryLSN
-      && frozenJournal.SeqEnd() <= SeqEnd()
-      && var freezed := FreezeOffRecent(keepReceiptLines);
-      && freezed.I().CanDiscardTo(frozenJournal.boundaryLSN)
-      && frozenJournal == freezed.DiscardOld(frozenJournal.boundaryLSN)
+      && OptRecCanCropHeadRecords(freshestRec, boundaryLSN, depth)
+      && CropHeadRecords(depth).I().CanDiscardTo(frozenJournal.boundaryLSN) // TODO(tony) remove I() here; replace with local condition
+      // probably want: CropHeadRecords(depth).seqStart <= frozenJournal.boundaryLSN
+      && frozenJournal == CropHeadRecords(depth).DiscardOldDefn(frozenJournal.boundaryLSN)
     }
   } // datatype TruncatedJournal
-
-  ////////////////////////////////////////////////////////////////////////////
-  // Receipt framework
-  //
-  // A Valid() Receipt is evidence that a JournalRecord does or does not
-  // contain a sensible linked list.
-  //
-  // A TJValid() Receipt is evidence that the JournalRecord DOES contain
-  // a sensible linked list.
-  //
-  // BuildReceipt is evidence that every TruncatedJournal has a Valid receipt.
-  //
-  // ReceiptsUnique says that any two Valid receipts for the same
-  //   TruncatedJournal are identical, so the one you Build matches the
-  //   one you get by snipping a line off of another receipt.
-  ////////////////////////////////////////////////////////////////////////////
-
-  datatype ReceiptLine = ReceiptLine(
-    journalRec: JournalRecord,
-    // None means the JournalRecord was malformed, at least with respect to the
-    // boundaryLSN.
-    interpretation: Option<MsgHistory>)
-  {
-    predicate WF() {
-      && journalRec.WF()
-      && (interpretation.Some? ==> interpretation.value.WF())
-    }
-
-    function Truncated(boundaryLSN: LSN) : MsgHistory
-      requires WF()
-    {
-      if journalRec.messageSeq.CanDiscardTo(boundaryLSN)
-      then journalRec.messageSeq.DiscardOld(boundaryLSN)
-      else journalRec.messageSeq
-    }
-
-    predicate Borked() { !journalRec.WF() }
-    predicate Unused(boundaryLSN: LSN) {
-      && journalRec.messageSeq.seqEnd <= boundaryLSN
-    }
-    predicate ListEnd() { journalRec.priorRec.None? }
-    predicate LineTJValid(boundaryLSN: LSN) {
-      // The record is well-formed, is a history, and includes the boundaryLSN.
-      && journalRec.WF()
-      && journalRec.messageSeq.seqStart <= boundaryLSN < journalRec.messageSeq.seqEnd
-    }
-
-    // A valid receipt either shows a valid TJ, or shows that the TJ starts in
-    // an invalid way.
-    predicate ValidFirstLine(boundaryLSN: LSN) {
-      || Borked()
-      || Unused(boundaryLSN)
-      || ListEnd()
-      || LineTJValid(boundaryLSN)
-    }
-
-    // A valid receipt doesn't have broken stuff in the middle. If something is
-    // wrong, it should be wrong at the top of the receipt
-    predicate ValidLaterLine(boundaryLSN: LSN) {
-      && journalRec.WF()
-      && boundaryLSN < journalRec.messageSeq.seqStart
-    }
-  }
-
-  datatype Receipt = Receipt(boundaryLSN: LSN, lines: seq<ReceiptLine>)
-  {
-    predicate LineRespectsLinkedList(i: nat)
-      requires 0<i<|lines|
-    {
-      && lines[i].journalRec.priorRec == Some(lines[i-1].journalRec)
-    }
-
-    predicate LinesRespectLinkedList()
-    {
-      forall i | 0<i<|lines| :: LineRespectsLinkedList(i)
-    }
-
-    predicate ValidLine(i: nat)
-      requires 0<=i<|lines|
-    {
-      if i==0 then lines[i].ValidFirstLine(boundaryLSN) else lines[i].ValidLaterLine(boundaryLSN)
-    }
-
-    predicate ValidLines()
-    {
-      forall i | 0<=i<|lines| :: ValidLine(i)
-    }
-
-    predicate InterpretationWF(i: nat)
-      requires i<|lines|
-    {
-      lines[i].interpretation.Some? ==> lines[i].interpretation.value.WF()
-    }
-
-    predicate InterpretationsWF()
-    {
-      forall i | 0<=i<|lines| :: InterpretationWF(i)
-    }
-
-    predicate FirstLineTJValid() {
-      0<|lines| ==> lines[0].LineTJValid(boundaryLSN)
-    }
-
-    function LinkedInterpretation(i: nat) : Option<MsgHistory>
-      requires InterpretationsWF()
-      requires i<|lines|
-    {
-      if !lines[i].WF()
-      then None // Bogus line
-      else if i==0
-      then (
-        if !FirstLineTJValid() then None else Some(lines[i].Truncated(boundaryLSN))
-      )
-      else if lines[i-1].interpretation.None?
-      then None // previous line already bogus
-      else if
-        assert InterpretationWF(i-1); // trigger
-        !lines[i-1].interpretation.value.CanConcat(lines[i].journalRec.messageSeq)
-      then None // adjacent lines don't stitch
-      else Some(lines[i-1].interpretation.value.Concat(lines[i].journalRec.messageSeq))
-    }
-
-    predicate OneLinkedInterpretation(i: nat)
-      requires InterpretationsWF()
-      requires i<|lines|
-    {
-      lines[i].interpretation == LinkedInterpretation(i)
-    }
-
-    predicate {:opaque} LinkedInterpretations() // TODO(jonh): can probably remove opaque now?
-      requires InterpretationsWF()
-    {
-      forall i | 0<=i<|lines| :: OneLinkedInterpretation(i)
-    }
-
-    // Valid means this receipt correctly explains the fate of the
-    // TruncatedJournal it represents, whether that be its interpretation
-    // or the fact that it's uninterpretable.
-    predicate Valid()
-    {
-      && LinesRespectLinkedList()
-      && ValidLines()
-      && InterpretationsWF()
-      && LinkedInterpretations()
-    }
-
-    // TJValid means the TruncatedJournal this receipt represents is itself
-    // valid -- it has a valid interpretation.
-    predicate TJValid()
-    {
-      && Valid()
-      // Final interpretation is happy.
-      && (0 < |lines| ==> && Last(lines).interpretation.Some?)
-    }
-
-    lemma SomeInterpretation(j: nat)
-      requires TJValid()
-      requires j <= |lines|
-      ensures forall i | j <= i < |lines| :: lines[i].interpretation.Some?
-      decreases |lines|-j
-    {
-      forall i | j <= i < |lines| ensures lines[i].interpretation.Some? {
-        if i < |lines|-1 {
-          SomeInterpretation(i + 1);  // i+1 is some by induction hypothesis
-          assert OneLinkedInterpretation(i+1) by { // if i were None, contradiction!
-            reveal_LinkedInterpretations();
-          }
-        }
-      }
-    }
-
-    lemma JournalRecsAllWF()
-      requires TJValid()
-      ensures forall i | 0<=i<|lines| :: lines[i].journalRec.WF()
-    {
-      SomeInterpretation(0);
-      forall i | 0<=i<|lines| ensures lines[i].journalRec.WF() {
-        assert InterpretationWF(i); // trigger
-        assert OneLinkedInterpretation(i) by { reveal_LinkedInterpretations(); }
-      }
-    }
-
-    // A package of popular facts about TJValid receipts.
-    lemma TJFacts()
-      requires TJValid()
-      ensures forall i | 0<=i<|lines| :: lines[i].interpretation.Some?
-      ensures forall i | 0<=i<|lines| :: lines[i].journalRec.WF()
-      ensures forall i | 0<=i<|lines| :: lines[i].interpretation.value.seqEnd == lines[i].journalRec.messageSeq.seqEnd
-      ensures FirstLineTJValid()
-      ensures I().seqStart == boundaryLSN
-      ensures I().WF()
-    {
-      SomeInterpretation(0);
-      JournalRecsAllWF();
-      if 0 < |lines| {
-        assert OneLinkedInterpretation(0) by { reveal_LinkedInterpretations(); }
-      }
-      forall i | 0<=i<|lines|
-        ensures lines[i].interpretation.value.seqEnd == lines[i].journalRec.messageSeq.seqEnd
-      {
-        if i>0 {
-          assert OneLinkedInterpretation(i) by { reveal_LinkedInterpretations(); }
-          assert InterpretationWF(i-1);
-        }
-      }
-      if 0<|lines| { assert InterpretationWF(|lines|-1); } // trigger to get I().WF()
-
-      var i:=0;
-      while i<|lines|
-        invariant i<=|lines|
-        invariant forall j:nat | j < i :: lines[j].interpretation.value.seqStart == boundaryLSN
-      {
-        assert OneLinkedInterpretation(i) by { reveal_LinkedInterpretations(); }
-        i:=i+1;
-      }
-    }
-
-    function I() : MsgHistory
-      requires TJValid()
-      ensures I().WF()
-    {
-      if |lines|==0
-      then EmptyHistoryAt(boundaryLSN)
-      else
-        var lastInterp := Last(lines).interpretation.value;
-        assert InterpretationWF(|lines|-1);
-        lastInterp
-    }
-
-    // Returns the message history represented by journal page i in this receipt
-    function MessageSeqAt(i: nat) : (out:MsgHistory)
-      requires i < |lines|
-      requires TJValid()  // maybe?
-      ensures out.WF()
-    {
-      var rec := lines[i].journalRec;
-      JournalRecsAllWF();
-      if rec.messageSeq.CanDiscardTo(boundaryLSN)
-      then rec.messageSeq.DiscardOld(boundaryLSN)
-      else rec.messageSeq
-    }
-
-    function SnipLast() : Receipt
-      requires 0 < |lines|
-    {
-      Receipt(boundaryLSN, DropLast(lines))
-    }
-
-    lemma SnippedReceiptValid()
-      requires Valid()
-      requires 0 < |lines|
-      ensures SnipLast().Valid()
-    {
-      // trigger party.
-      forall i | 0<i<|lines|-1 ensures SnipLast().LineRespectsLinkedList(i) {
-        assert LineRespectsLinkedList(i);
-      }
-      reveal_LinkedInterpretations();
-      forall i | 0<=i<|lines|-1
-        ensures SnipLast().ValidLine(i)
-        ensures SnipLast().InterpretationWF(i)
-        ensures SnipLast().OneLinkedInterpretation(i)
-      {
-        assert ValidLine(i);
-        assert InterpretationWF(i);
-        assert OneLinkedInterpretation(i);
-      }
-    }
-
-    // You can snip the end off of a TJValid receipt and what's left is still valid.
-    // (This is a way to construct a TJValid receipt other than BuildReceipt.)
-    lemma SnippedReceiptTJValid()
-      requires TJValid()
-      requires 0 < |lines|
-      ensures SnipLast().TJValid()
-    {
-      SnippedReceiptValid();
-      assert OneLinkedInterpretation(|lines|-1) by { reveal_LinkedInterpretations(); }
-    }
-
-    function SnipAt(keepReceiptLines: nat) : Receipt
-      requires keepReceiptLines <= |lines|
-    {
-      Receipt(boundaryLSN, lines[..keepReceiptLines])
-    }
-  
-    lemma SnipAtTJValid(keepReceiptLines: nat)
-      requires TJValid()
-      requires keepReceiptLines <= |lines|
-      ensures SnipAt(keepReceiptLines).TJValid()
-      decreases |lines|
-    {
-      if keepReceiptLines==|lines| {
-        assert SnipAt(keepReceiptLines) == this;  // seq trigger
-      } else {
-        SnippedReceiptTJValid();
-        if keepReceiptLines < |lines|-1 {
-          assert SnipLast().SnipAt(keepReceiptLines) == SnipAt(keepReceiptLines); // seq trigger
-          SnipLast().SnipAtTJValid(keepReceiptLines);
-        }
-      }
-    }
-
-    function FreshestRec() : Option<JournalRecord>
-    {
-      if |lines|==0 then None else Some(Last(lines).journalRec)
-    }
-
-    function TJ() : TruncatedJournal
-    {
-      TruncatedJournal(boundaryLSN, FreshestRec())
-    }
-
-    lemma ReceiptsUnique(r2: Receipt)
-      requires Valid()
-      requires r2.Valid()
-      requires TJ() == r2.TJ()
-      ensures this == r2
-      decreases |lines|
-    {
-      if |lines| == 0 {
-        // assert this == r2;  // case boilerplate
-      } else {
-        SnippedReceiptValid();
-        r2.SnippedReceiptValid();
-        assert OneLinkedInterpretation(|lines|-1) by { reveal_LinkedInterpretations(); }
-        assert r2.OneLinkedInterpretation(|r2.lines|-1) by { reveal_LinkedInterpretations(); }
-
-        if 1==|lines| && 1==|r2.lines| {
-          // assert this == r2;  // case boilerplate
-        } else if 1==|lines| {
-          // If I'm out of records, r2 can't keep going.
-          assert r2.LineRespectsLinkedList(|r2.lines|-1); // trigger
-          assert ValidLine(0);  // trigger
-          assert !r2.ValidLine(|r2.lines|-1); // witness to contradiction
-        } else if 1==|r2.lines| {
-          // symmetric impossible case
-          assert LineRespectsLinkedList(|lines|-1); // trigger
-          assert r2.ValidLine(0);  // trigger
-          assert !ValidLine(|lines|-1); // witness to contradiction
-        } else {
-          // recurse
-          assert r2.LineRespectsLinkedList(|r2.lines|-1); // trigger
-          assert LineRespectsLinkedList(|lines|-1); // trigger
-          SnipLast().ReceiptsUnique(r2.SnipLast()); // recurse
-          // assert this == r2;  // case boilerplate
-        }
-      }
-    }
-
-    lemma AbbreviatedReceiptTJValid(i: nat, endLsn: LSN, tj: TruncatedJournal)
-      requires TJValid()
-      requires i < |lines|
-      requires
-        assert lines[i].journalRec.WF() by { TJFacts(); }
-        endLsn == lines[i].journalRec.messageSeq.seqEnd
-      requires tj == TruncatedJournal(boundaryLSN, Some(lines[i].journalRec))
-      ensures tj.WF()
-      ensures I().WF()
-      ensures I().CanDiscardTo(endLsn)
-      ensures tj.I() == I().DiscardRecent(endLsn)
-      decreases |lines|
-    {
-      TJFacts();
-      assert OneLinkedInterpretation(|lines|-1) by { reveal_LinkedInterpretations(); }
-      if i == |lines| - 1 {
-        // Receipt for same TJ -> same receipt!
-        ReceiptsUnique(tj.BuildReceipt());
-      } else if i == |lines|-2 {  
-        // just dropping one row from receipt?
-        SnippedReceiptTJValid();
-        if 1<|lines| {
-          tj.BuildReceipt().ReceiptsUnique(SnipLast());
-        }
-      } else {
-        // Dropping many rows; induct.
-        SnippedReceiptTJValid();
-        SnipLast().AbbreviatedReceiptTJValid(i, endLsn, tj);
-      }
-    }
-
-    lemma BoundaryLSN()
-      requires TJValid()
-      ensures I().seqStart == boundaryLSN
-      ensures !I().IsEmpty() ==> FreshestRec().Some?  // from TJFacts
-      ensures !I().IsEmpty() ==> I().seqEnd == FreshestRec().value.messageSeq.seqEnd
-    {
-      TJFacts();
-      var i:nat := 0;
-      while i<|lines|
-        invariant i<=|lines|
-        invariant forall j | 0<=j<i :: lines[j].interpretation.value.seqStart == boundaryLSN
-      {
-        assert OneLinkedInterpretation(i) by { reveal_LinkedInterpretations(); }
-        i := i + 1;
-      }
-    }
-
-    lemma DiscardOld(lsn: LSN) returns (out:Receipt)
-      requires TJValid()
-      requires I().CanDiscardTo(lsn)
-      ensures out.TJValid()
-      ensures I().WF()
-      ensures TJ().WF() // just TJValid + ReceiptsUnique
-      ensures TJ().I().CanDiscardTo(lsn);
-      ensures out.TJ() == TJ().DiscardOldDefn(lsn)
-      ensures out.I() == I().DiscardOld(lsn)
-      decreases |lines|
-    {
-      TJFacts();
-      BoundaryLSN();
-      ReceiptsUnique(TJ().BuildReceipt());
-      if I().IsEmpty() || lsn==I().seqEnd {   // Output receipt is entirely empty
-        out := Receipt(lsn, []);
-        assert out.TJValid() by { reveal_LinkedInterpretations(); }
-        assert out.I() == I().DiscardOld(lsn);  // case boilerplate
-      } else if Last(lines).journalRec.messageSeq.seqStart <= lsn { // Discarding something in last, but keeping some of it
-        var outRec := JournalRecord(Last(lines).journalRec.messageSeq, None);
-        out := Receipt(lsn, [ReceiptLine(outRec, Some(outRec.messageSeq.DiscardOld(lsn)))]);
-        assert out.LinkedInterpretations() by { reveal_LinkedInterpretations(); }
-        // This is the top of the new receipt
-        assert OneLinkedInterpretation(|lines|-1) by { reveal_LinkedInterpretations(); }
-        assert out.I() == I().DiscardOld(lsn);  // case boilerplate
-      } else {  // Recurse
-        SnippedReceiptTJValid();
-        assert OneLinkedInterpretation(|lines|-1) by { reveal_LinkedInterpretations(); }
-        var shortReceipt := SnipLast().DiscardOld(lsn); // here's the recursive call.
-        // Tack on the last line.
-        var lastInterp := shortReceipt.I().Concat(Last(lines).journalRec.messageSeq);
-        var lastRecordDiscarded := DiscardOldJournalRec(Some(Last(lines).journalRec), lsn).value;
-        out := Receipt(lsn, shortReceipt.lines + [ReceiptLine(lastRecordDiscarded, Some(lastInterp))]);
-
-        // trigger party for automation-controlled Valid quantifiers
-        forall i | 0<i<|out.lines| ensures out.LineRespectsLinkedList(i) {
-          if i < |out.lines|-1 {
-            assert shortReceipt.LineRespectsLinkedList(i);  // induction hypothesis
-          } else {
-            assert LineRespectsLinkedList(|lines|-1);       // new line
-          }
-        }
-        forall i | 0<=i<|out.lines|
-          ensures out.ValidLine(i)
-          ensures out.InterpretationWF(i)
-          ensures out.OneLinkedInterpretation(i)
-        {
-          if i < |out.lines|-1 {
-            assert shortReceipt.ValidLine(i);
-            assert shortReceipt.InterpretationWF(i);
-            assert shortReceipt.OneLinkedInterpretation(i) by { reveal_LinkedInterpretations(); }
-          }
-        }
-        assert out.Valid() by { reveal_LinkedInterpretations(); }
-        assert out.I() == I().DiscardOld(lsn);  // case boilerplate
-      }
-    }
-
-    lemma LsnInReceiptBelongs(i: nat)
-      requires TJValid()
-      requires i < |lines|
-      ensures lines[i].WF()
-      ensures I().CanDiscardTo(lines[i].journalRec.messageSeq.seqEnd)
-      decreases |lines|
-    {
-      TJFacts();
-      assert OneLinkedInterpretation(i) by { reveal_LinkedInterpretations(); }
-      if i<|lines|-1 {
-        SnippedReceiptTJValid();  // recurse
-        SnipLast().LsnInReceiptBelongs(i);
-        assert OneLinkedInterpretation(|lines|-1) by { reveal_LinkedInterpretations(); }
-      }
-    }
-  } // datatype Receipt
-
-  // Constructive evidence that a Valid receipt exists for each TJ
-  function BuildReceiptRecursive(boundaryLSN: LSN, optRec: Option<JournalRecord>) : (out:Receipt)
-    ensures out.Valid()
-  {
-    // A global Receipt(0,[]).reveal_LinkedInterpretations() makes this function
-    // prove, but because this function's body is reachable from WF, pollutes
-    // lots of later CheckWellformeds to run out of resource.
-    if optRec.None?
-    then var out := Receipt(boundaryLSN, []);
-      assert out.Valid() by { Receipt(0,[]).reveal_LinkedInterpretations(); }
-      out
-    else
-      var rec := optRec.value;
-      if !rec.WF()
-      then
-        // Malformed record
-        var out := Receipt(boundaryLSN, [ReceiptLine(rec, None)]);
-        assert out.Valid() by { Receipt(0,[]).reveal_LinkedInterpretations(); }
-        out
-      else if rec.messageSeq.seqEnd <= boundaryLSN
-      then
-        // Uh, this journal record ends before boundaryLSN? Why do we have it?
-        var out := Receipt(boundaryLSN, [ReceiptLine(rec, None)]);
-        assert out.Valid() by { Receipt(0,[]).reveal_LinkedInterpretations(); }
-        out
-      else if rec.messageSeq.seqStart <= boundaryLSN
-      then
-        // boundaryLSN satisfied here; can stop decoding. Don't care what lies
-        // beyond!
-        var out := Receipt(boundaryLSN, [ReceiptLine(rec, Some(rec.messageSeq.DiscardOld(boundaryLSN)))]);
-        assert out.Valid() by { Receipt(0,[]).reveal_LinkedInterpretations(); }
-        out
-      else if rec.priorRec.None?
-      then (
-        assert boundaryLSN < rec.messageSeq.seqStart;
-        // Uh oh, we needed a prior rec!
-        var out := Receipt(boundaryLSN, [ReceiptLine(rec, None)]);
-        assert out.Valid() by { Receipt(0,[]).reveal_LinkedInterpretations(); }
-        out
-      )
-      else
-        // Recurse.
-        var priorReceipt := BuildReceiptRecursive(boundaryLSN, rec.priorRec);
-        var priorInterpretation := Last(priorReceipt.lines).interpretation;
-        var newInterpretation :=
-          if
-            // Recursion was invalid
-            || priorInterpretation.None?
-            // Or didn't stitch.
-            || !priorInterpretation.value.CanConcat(rec.messageSeq)
-          then None
-          else Some(priorReceipt.I().Concat(rec.messageSeq));
-        var out := Receipt(boundaryLSN,
-          priorReceipt.lines + [ReceiptLine(rec, newInterpretation)]);
-        assert out.Valid() by {
-          // trigger some features of the base case lines
-          forall i | 0<=i<|out.lines|
-            ensures out.InterpretationWF(i)
-            ensures out.ValidLine(i)
-          {
-            if i<|out.lines|-1 {
-              assert priorReceipt.InterpretationWF(i);
-              assert priorReceipt.ValidLine(i);
-            }
-          }
-          forall i | 0<i<|out.lines| ensures out.LineRespectsLinkedList(i) {
-            if i<|out.lines|-1 {
-              assert priorReceipt.LineRespectsLinkedList(i);
-            }
-          }
-          assert out.LinkedInterpretations() by {
-            out.reveal_LinkedInterpretations();
-            forall i | 0<=i<|out.lines| ensures out.OneLinkedInterpretation(i) {
-              if i<|out.lines|-1 {
-                assert priorReceipt.OneLinkedInterpretation(i);
-              }
-            }
-          }
-        }
-        out
-  } // BuildReceiptRecursive
 
   // TruncatedJournal is the datatype "refinement" of MsgHistory; here we refine the Mkfs function.
   function Mkfs() : (out:TruncatedJournal)
@@ -792,7 +276,6 @@ module PagedJournal {
       requires WF()
       ensures SeqStart() == I().seqStart
     {
-      truncatedJournal.BuildReceipt().TJFacts();
       truncatedJournal.boundaryLSN
     }
 
@@ -803,12 +286,12 @@ module PagedJournal {
     }
   }
 
-  predicate ReadForRecovery(v: Variables, v': Variables, lbl: TransitionLabel, receiptIndex: nat)
+  predicate ReadForRecovery(v: Variables, v': Variables, lbl: TransitionLabel, depth: nat)
   {
     && v.WF()
     && lbl.ReadForRecoveryLabel?
     && lbl.messages.WF()
-    && v.truncatedJournal.IncludesSubseqAt(lbl.messages, receiptIndex) // subseq appears in committed pages
+    && v.truncatedJournal.HasMessagesAtDepth(lbl.messages, depth) // subseq appears in committed pages
     && v' == v
 
     // We don't bother allowing you to "find" the msgs in unmarshalledTail,
@@ -866,7 +349,7 @@ module PagedJournal {
           assert lsn <= v.unmarshalledTail.seqEnd;
           Variables(TruncatedJournal(lsn, None), v.unmarshalledTail.DiscardOld(lsn))
         else
-          v.(truncatedJournal := v.truncatedJournal.DiscardOld(lsn))
+          v.(truncatedJournal := v.truncatedJournal.DiscardOldDefn(lsn))
        )
   }
 
